1 final lemma for the representation.

MirrorCharge!/src/Cancel.v
@@ -1,11 +1,9 @@
 (** This file implements cancellation for separation logic.
- **
- ** Phase 1)
- ** - Support star and emp
  **)
 Require Import ExtLib.Data.Positive.
+Require Import ExtLib.Data.HList.
 Require Import ExtLib.Tactics.
-Require Import BILogic.
+Require Import BILogic ILogic Pure.
 Require Import MirrorCore.EnvI.
 Require Import MirrorCore.SymI.
 Require Import MirrorCore.Ext.Expr.
@@ -15,50 +13,994 @@ Require Import ILogicFunc SepLogFold.
 Set Implicit Arguments.
 Set Strict Implicit.
 
+Section iterated.
+  Variable T : Type.
+  Variable base : T.
+  Variable join : T -> T -> T.
+
+  Fixpoint iterated (ls : list T) : option T :=
+    match ls with
+      | nil => None
+      | l :: ls => match iterated ls with
+                     | None => Some l
+                     | Some ls => Some (join l ls)
+                   end
+    end.
+
+  Definition iterated_base (ls : list T) : T :=
+    match iterated ls with
+      | None => base
+      | Some l => l
+    end.
+
+  Lemma iterated_None : forall ls, iterated ls = None -> ls = nil.
+  Proof.
+    destruct ls; simpl; intros; try congruence.
+    destruct (iterated ls); congruence.
+  Qed.
+
+  Require Import Relations Morphisms.
+  Require Import RelationClasses.
+
+  Hypothesis R : relation T.
+  Hypothesis Reflexive_R : Reflexive R.
+  Hypothesis Transitive_R : Transitive R.
+  Hypothesis join_assoc : forall a b c, R (join a (join b c)) (join (join a b) c).
+  Hypothesis join_respects : Proper (R ==> R ==> R)%signature join.
+
+  Definition option_R (a b : option T) : Prop :=
+    match a , b with
+      | None , None => True
+      | Some a , Some b => R a b
+      | _ , _ => False
+    end.
+
+  Local Instance Reflexive_optionR : Reflexive option_R.
+  Proof.
+    red. destruct x; simpl; reflexivity.
+  Qed.
+  Local Instance Transitive_optionR : Transitive option_R.
+  Proof.
+    red. destruct x; destruct y; destruct z; simpl; intros; auto.
+    etransitivity; eauto. intuition.
+  Qed.
+
+  Theorem iterated_app
+  : forall ls' ls,
+      option_R (iterated (ls ++ ls'))
+               (match iterated ls' with
+                  | None => iterated ls
+                  | Some ls' => match iterated ls with
+                                  | None => Some ls'
+                                  | Some ls => Some (join ls ls')
+                                end
+                end).
+  Proof.
+    induction ls; simpl.
+    { intros. destruct (iterated ls'); reflexivity. }
+    { intros. unfold option_R in *.
+      repeat match goal with
+               | |- context [ match ?X with _ => _ end ] =>
+                 consider X; intros; try congruence
+               | H : context [ match ?X with _ => _ end ] |- _ =>
+                 consider X; intros; try congruence
+               | H : R _ _ |- _ => rewrite H
+             end; inv_all; subst; try solve [ congruence | intuition ].
+      { rewrite IHls. etransitivity. 2: eapply join_assoc. reflexivity. }
+      { rewrite H5. reflexivity. }
+      { rewrite H4; reflexivity. }
+      { subst. reflexivity. } }
+  Qed.
+
+
+  Hypothesis Rbase_LL : forall a, R (join base a) a.
+  Hypothesis Rbase_LR : forall a, R (join a base) a.
+  Hypothesis Rbase_RL : forall a, R a (join base a).
+  Hypothesis Rbase_RR : forall a, R a (join a base).
+
+  Theorem iterated_base_app
+  : forall ls' ls,
+      R (iterated_base (ls ++ ls'))
+        (join (iterated_base ls) (iterated_base ls')).
+  Proof.
+    induction ls; simpl.
+    { intros. unfold iterated_base. simpl.
+      eapply Rbase_RL. }
+    { unfold iterated_base in *; simpl in *.
+      destruct (iterated (ls ++ ls')).
+      { rewrite IHls.
+        rewrite join_assoc.
+        destruct (iterated ls); try reflexivity.
+        rewrite Rbase_LR. reflexivity. }
+      { destruct (iterated ls); destruct (iterated ls'); simpl.
+        { rewrite <- join_assoc. rewrite <- IHls. eapply Rbase_RR. }
+        { rewrite <- join_assoc. rewrite <- IHls. apply Rbase_RR. }
+        { rewrite Rbase_LL in IHls.
+          rewrite <- IHls. apply Rbase_RR. }
+        { eapply Rbase_RR. } } }
+  Qed.
+
+  Variable P : T -> Prop.
+  Hypothesis Pjoin : forall a b, P a -> P b -> P (join a b).
+
+  Theorem iterated_inv
+  : forall ls,
+      List.Forall P ls ->
+      match iterated ls with
+        | None => ls = nil
+        | Some e => P e
+      end.
+  Proof.
+    clear - Pjoin. induction 1; simpl; intros; auto.
+    destruct (iterated l); auto.
+  Qed.
+
+  Hypothesis Pbase : P base.
+
+  Theorem iterated_base_inv
+  : forall ls,
+      List.Forall P ls ->
+      P (iterated_base ls).
+  Proof.
+    clear - Pjoin Pbase.
+    unfold iterated_base; intros.
+    eapply iterated_inv in H. destruct (iterated ls); eauto.
+  Qed.
+
+End iterated.
+
 Section cancel_state.
+  Variable ts : types.
+  Variable sym : Type.
+  Variable RSym_sym : RSym (typD ts) sym.
+
   Record conjunctives : Type :=
-  { spacial : list (expr ilfunc * list (expr ilfunc)) }.
+  { spatial : option (list (expr sym * list (expr sym)))
+  ; pure : list (expr sym)
+  }.
 
-  Definition empty : conjunctives :=
-    {| spacial := nil |}.
+  Definition mkEmpty : conjunctives :=
+  {| spatial := Some (nil)
+   ; pure := nil
+   |}.
 
-  Definition atomic e : conjunctives :=
-    {| spacial := app_full e :: nil |}.
+  Definition mkPure e : conjunctives :=
+  {| spatial := None
+   ; pure := e :: nil
+   |}.
 
-  Definition atomic_app e es : conjunctives :=
-    {| spacial := (e, es) :: nil |}.
+  Definition mkSpatial e es : conjunctives :=
+  {| spatial := Some ((e,es) :: nil)
+   ; pure := nil
+   |}.
 
-  Definition join (l r : conjunctives) : conjunctives :=
-    {| spacial := l.(spacial) ++ r.(spacial) |}.
+  Definition mkStar (l r : conjunctives) : conjunctives :=
+  {| spatial := match l.(spatial)  with
+                  | None => r.(spatial)
+                  | Some a => match r.(spatial) with
+                                | None => Some a
+                                | Some b => Some (a ++ b)
+                              end
+                end
+   ; pure := l.(pure) ++ r.(pure)
+   |}.
 
-  Definition is_emp (i : ilfunc) : bool :=
+  Definition SepLogArgs_normalize : SepLogArgs sym conjunctives :=
+  {| do_emp := mkEmpty
+   ; do_star := mkStar
+   ; do_atomic_app := mkSpatial
+   ; do_pure := mkPure
+   |}.
+
+  Variable SL : typ.
+
+  Section conjunctivesD.
+    Variable SLS : SepLogSpec sym.
+    Variable ILO : ILogicOps (typD ts nil SL).
+    Variable BILO : BILOperators (typD ts nil SL).
+    Variable IL : @ILogic _ ILO.
+    Variable BIL : @BILogic _ ILO BILO.
+
+    Variable slsok : SepLogSpecOk RSym_sym SL SLS ILO BILO.
+
+    Variable e_star : expr sym -> expr sym -> expr sym.
+    Variable e_and : expr sym -> expr sym -> expr sym.
+    Variable e_emp : expr sym.
+    Variable e_true : expr sym.
+
+    Definition well_formed (c : conjunctives) (us vs : env (typD ts)) : Prop :=
+      List.Forall (fun e =>
+                     exists val, exprD us vs e SL = Some val
+                              /\ @Pure.pure _ slsok.(_PureOp) val) c.(pure).
+
+    Definition conjunctives_to_expr (c : conjunctives) : expr sym :=
+      match c.(spatial) with
+        | None => iterated_base e_true e_and c.(pure)
+        | Some s =>
+          let s := iterated_base e_emp e_star (map (fun x => apps (fst x) (snd x)) s) in
+          match iterated e_and c.(pure) with
+            | None => s
+            | Some p => e_and p s
+          end
+      end.
+
+    Definition conjunctives_to_expr' (c : conjunctives) : expr sym :=
+      let spa :=
+          match c.(spatial) with
+            | None => e_true
+            | Some s => iterated_base e_emp e_star (map (fun x => apps (fst x) (snd x)) s)
+          end
+      in
+      let pur := iterated_base e_true e_and c.(pure) in
+      e_and pur spa.
+
+    Definition R_conjunctives
+               (e : expr sym) (c : conjunctives) (tus tvs : tenv typ) : Prop :=
+      forall us : hlist _ tus,
+      forall val,
+        exprD' (ts := ts) (join_env us) tvs e SL = Some val ->
+        exists val',
+             exprD' (join_env us) tvs (conjunctives_to_expr c) SL = Some val'
+          /\ (forall vs, 
+                (val vs -|- val' vs) /\ well_formed c (join_env us) (join_env vs)).
+
+    Hypothesis e_empOk : forall us tvs,
+                         exists val,
+                           exprD' us tvs e_emp SL = Some val /\
+                           forall vs, val vs -|- empSP.
+    Hypothesis e_trueOk : forall us tvs,
+                          exists val,
+                            exprD' us tvs e_true SL = Some val /\
+                            forall vs, val vs -|- ltrue.
+    Hypothesis e_starOk : forall us tvs x y valx valy,
+                            exprD' us tvs x SL = Some valx ->
+                            exprD' us tvs y SL = Some valy ->
+                            exists val,
+                              exprD' us tvs (e_star x y) SL = Some val /\
+                              forall vs, val vs -|- valx vs ** valy vs.
+    Hypothesis e_starValid : forall us tvs x y val,
+                               exprD' us tvs (e_star x y) SL = Some val ->
+                               exists valx valy,
+                                 exprD' us tvs x SL = Some valx /\
+                                 exprD' us tvs y SL = Some valy /\
+                                 forall vs, val vs -|- valx vs ** valy vs.
+    Hypothesis e_andOk : forall us tvs x y valx valy,
+                            exprD' us tvs x SL = Some valx ->
+                            exprD' us tvs y SL = Some valy ->
+                            exists val,
+                              exprD' us tvs (e_and x y) SL = Some val /\
+                              forall vs, val vs -|- valx vs //\\ valy vs.
+    Hypothesis e_andValid : forall us tvs x y val,
+                              exprD' us tvs (e_and x y) SL = Some val ->
+                              exists valx valy,
+                                exprD' us tvs x SL = Some valx /\
+                                exprD' us tvs y SL = Some valy /\
+                                forall vs, val vs -|- valx vs //\\ valy vs.
+
+    Ltac forward_ex_and :=
+      repeat match goal with
+               | H : exists x, _ |- _ => destruct H
+               | H : _ /\ _ |- _ => destruct H
+             end.
+
+    Lemma e_andOk_None1
+    : forall us tvs x y,
+        exprD' us tvs x SL = None ->
+        exprD' us tvs (e_and x y) SL = None.
+    Proof.
+      intros.
+      consider (exprD' us tvs (e_and x y) SL); auto; intros.
+      exfalso.
+      eapply e_andValid in H0. forward_ex_and. congruence.
+    Qed.
+
+    Lemma e_andOk_None2
+    : forall us tvs x y,
+        exprD' us tvs y SL = None ->
+        exprD' us tvs (e_and x y) SL = None.
+    Proof.
+      intros.
+      consider (exprD' us tvs (e_and x y) SL); auto; intros.
+      exfalso.
+      eapply e_andValid in H0. forward_ex_and. congruence.
+    Qed.
+
+    Lemma e_starOk_None1
+    : forall us tvs x y,
+        exprD' us tvs x SL = None ->
+        exprD' us tvs (e_star x y) SL = None.
+    Proof.
+      intros.
+      consider (exprD' us tvs (e_star x y) SL); auto; intros.
+      exfalso.
+      eapply e_starValid in H0. forward_ex_and. congruence.
+    Qed.
+
+    Lemma e_starOk_None2
+    : forall us tvs x y,
+        exprD' us tvs y SL = None ->
+        exprD' us tvs (e_star x y) SL = None.
+    Proof.
+      intros.
+      consider (exprD' us tvs (e_star x y) SL); auto; intros.
+      exfalso.
+      eapply e_starValid in H0. forward_ex_and. congruence.
+    Qed.
+
+    Definition Sem_ext (t : typ) (P : typD ts nil t -> Prop) (Q : Prop)
+    : expr sym -> Prop :=
+      fun e =>
+        forall us tvs,
+          match exprD' us tvs e t with
+            | Some val =>
+              forall vs, P (val vs)
+            | None => Q
+          end.
+
+    Ltac go_crazy :=
+      match goal with
+        | H : exprD' _ _ _ _ = _ , H' : _ |- _ =>
+          rewrite H in H'
+        | H : exprD' _ _ _ _ = _ |- _ =>
+          rewrite H
+        | H : exprD' _ _ (e_and _ _) _ = _ |- _ =>
+          eapply e_andValid in H ; destruct H as [ ? [ ? [ ? [ ? ? ] ] ] ]
+        | H : exprD' _ _ (e_star _ _) _ = _ |- _ =>
+          eapply e_starValid in H ; destruct H as [ ? [ ? [ ? [ ? ? ] ] ] ]
+        | H : exprD' _ _ ?C _ = _
+        , H' : exprD' _ _ ?D _ = _
+        |- context [ exprD' ?A ?B (e_and ?C ?D) ?T ] =>
+          destruct (@e_andOk _ _ _ _ _ _ H H') as [ ? [ ? ? ] ]
+        | H : exprD' _ _ ?C _ = _
+        , H' : exprD' _ _ ?D _ = _
+        |- context [ exprD' ?A ?B (e_star ?C ?D) ?T ] =>
+          destruct (@e_starOk _ _ _ _ _ _ H H') as [ ? [ ? ? ] ]
+        | H : exprD' _ _ ?C _ = _
+        , H' : exprD' _ _ ?D _ = _
+        , H'' : context [ exprD' ?A ?B (e_star ?C ?D) ?T ]
+        |- _ =>
+          destruct (@e_starOk _ _ _ _ _ _ H H') as [ ? [ ? ? ] ]
+        | H : exprD' _ _ ?C _ = _
+        , H' : exprD' _ _ ?D _ = _
+        , H'' : context [ exprD' ?A ?B (e_and ?C ?D) ?T ]
+        |- _ =>
+          destruct (@e_andOk _ _ _ _ _ _ H H') as [ ? [ ? ? ] ]
+        | H : exprD' _ _ _ _ = None |- _ =>
+          first [ erewrite (@e_starOk_None1 _ _ _ _ H) in *
+                | erewrite (@e_starOk_None2 _ _ _ _ H) in *
+                | erewrite (@e_andOk_None1 _ _ _ _ H) in *
+                | erewrite (@e_andOk_None2 _ _ _ _ H) in * ]
+      end.
+
+    Local Instance Reflexive_lentails : Reflexive lentails.
+    Proof.
+      destruct IL. destruct lentailsPre. auto.
+    Qed.
+
+    Require Import MirrorCore.Ext.ExprSem.
+
+    Theorem conjunctives_to_expr_conjunctives_to_expr'
+    : forall e,
+        Sem_equiv _ SL lequiv (conjunctives_to_expr e) (conjunctives_to_expr' e).
+    Proof.
+      destruct e.
+      unfold conjunctives_to_expr, conjunctives_to_expr', iterated_base; simpl.
+      generalize (iterated e_and pure0); intros.
+      destruct spatial0.
+      { generalize (iterated e_star
+                             (map
+                                (fun x : expr sym * list (expr sym) =>
+                                   apps (fst x) (snd x)) l)).
+        intro.
+        generalize (match o0 with
+                      | Some l0 => l0
+                      | None => e_emp
+                    end); intro.
+        red. intros.
+        destruct o.
+        { forward. reflexivity. }
+        { destruct (e_trueOk us tvs). destruct H.
+          consider (exprD' us tvs e SL); intros; repeat go_crazy; auto.
+          inv_all; subst. intros. rewrite H3. rewrite H0.
+          rewrite landtrueL. reflexivity. } }
+      { red. intros.
+        generalize (match o with
+                      | Some l => l
+                      | None => e_true
+                    end); intros.
+        destruct (e_trueOk us tvs). destruct H.
+        consider (exprD' us tvs e SL); intros; repeat go_crazy; auto.
+        inv_all; subst. intros.
+        rewrite H5. rewrite H0. rewrite landtrueR. reflexivity. }
+    Qed.
+
+    Lemma Sem_equiv_e_and_assoc
+    : forall a b c : expr sym,
+        Sem_equiv _ SL lequiv (e_and a (e_and b c)) (e_and (e_and a b) c).
+    Proof.
+      clear - IL e_andOk e_andValid. intros.
+      red. intros.
+      consider (exprD' us tvs (e_and a (e_and b c)) SL);
+        consider (exprD' us tvs (e_and (e_and a b) c) SL); intros; auto.
+      { eapply e_andValid in H. eapply e_andValid in H0.
+        do 2 destruct H; do 2 destruct H0.
+        destruct H0. destruct H1. destruct H. destruct H3.
+        eapply e_andValid in H. do 3 destruct H. destruct H5.
+        eapply e_andValid in H1. do 3 destruct H1. destruct H7.
+        rewrite H4. rewrite H2. rewrite H6. rewrite H8.
+        rewrite H0 in *. rewrite H5 in *. rewrite H7 in *.
+        inv_all; subst.
+        symmetry. eapply landA. }
+      { eapply e_andValid in H0.
+        do 3 destruct H0. destruct H1.
+        eapply e_andValid in H1.
+        do 3 destruct H1. destruct H3.
+        destruct (@e_andOk _ _ _ _ _ _ H0 H1). destruct H5.
+        destruct (@e_andOk _ _ _ _ _ _ H5 H3). destruct H7.
+        congruence. }
+      { eapply e_andValid in H.
+        do 3 destruct H. destruct H1.
+        eapply e_andValid in H.
+        do 3 destruct H. destruct H3.
+        destruct (@e_andOk _ _ _ _ _ _ H3 H1). destruct H5.
+        destruct (@e_andOk _ _ _ _ _ _ H H5). destruct H7.
+        congruence. }
+    Qed.
+
+    Lemma Sem_equiv_e_star_assoc
+    : forall a b c : expr sym,
+        Sem_equiv _ SL lequiv (e_star a (e_star b c)) (e_star (e_star a b) c).
+    Proof.
+      clear - IL BIL e_starOk e_starValid. intros.
+      red. intros.
+      consider (exprD' us tvs (e_star a (e_star b c)) SL);
+        consider (exprD' us tvs (e_star (e_star a b) c) SL); intros; auto.
+      { eapply e_starValid in H. eapply e_starValid in H0.
+        do 2 destruct H; do 2 destruct H0.
+        destruct H0. destruct H1. destruct H. destruct H3.
+        eapply e_starValid in H. do 3 destruct H. destruct H5.
+        eapply e_starValid in H1. do 3 destruct H1. destruct H7.
+        rewrite H4. rewrite H2. rewrite H6. rewrite H8.
+        rewrite H0 in *. rewrite H5 in *. rewrite H7 in *.
+        inv_all; subst.
+        symmetry. eapply sepSPA. }
+      { eapply e_starValid in H0.
+        do 3 destruct H0. destruct H1.
+        eapply e_starValid in H1.
+        do 3 destruct H1. destruct H3.
+        destruct (@e_starOk _ _ _ _ _ _ H0 H1). destruct H5.
+        destruct (@e_starOk _ _ _ _ _ _ H5 H3). destruct H7.
+        congruence. }
+      { eapply e_starValid in H.
+        do 3 destruct H. destruct H1.
+        eapply e_starValid in H.
+        do 3 destruct H. destruct H3.
+        destruct (@e_starOk _ _ _ _ _ _ H3 H1). destruct H5.
+        destruct (@e_starOk _ _ _ _ _ _ H H5). destruct H7.
+        congruence. }
+    Qed.
+
+    Lemma Sem_equiv_Proper_e_and
+    : Proper (Sem_equiv _ SL lequiv ==> Sem_equiv _ SL lequiv ==> Sem_equiv _ SL lequiv) e_and.
+    Proof.
+      unfold Sem_equiv; repeat red; simpl; intros.
+      specialize (H us tvs). specialize (H0 us tvs).
+      match goal with
+        | |- match ?X with _ => _ end =>
+          consider X; intros
+      end; repeat go_crazy; forward; repeat go_crazy.
+      { inv_all; subst.
+        intros. rewrite H3. rewrite H4. rewrite H9.
+        rewrite H5. reflexivity. }
+      { forward.
+        go_crazy. congruence. }
+    Qed.
+
+    Lemma Sem_equiv_Proper_e_star
+    : Proper (Sem_equiv _ SL lequiv ==> Sem_equiv _ SL lequiv ==> Sem_equiv _ SL lequiv) e_star.
+    Proof.
+      unfold Sem_equiv; repeat red; simpl; intros.
+      specialize (H us tvs). specialize (H0 us tvs).
+      match goal with
+        | |- match ?X with _ => _ end =>
+          consider X; intros
+      end; repeat go_crazy; forward; repeat go_crazy.
+      { inv_all; subst.
+        intros. rewrite H3. rewrite H4. rewrite H9.
+        rewrite H5. reflexivity. }
+      { forward.
+        go_crazy. congruence. }
+    Qed.
+
+    Lemma ltrue_unitL : forall a, land ltrue a -|- a.
+    Proof.
+      clear - IL; intros.
+      split.
+      { eapply landL2. reflexivity. }
+      { eapply landR; try reflexivity. eapply ltrueR. }
+    Qed.
+
+    Lemma ltrue_unitR : forall a, land a ltrue -|- a.
+    Proof.
+      clear - IL; intros.
+      split.
+      { eapply landL1. reflexivity. }
+      { eapply landR; try reflexivity. eapply ltrueR. }
+    Qed.
+
+    Lemma empSPR : forall a, a ** empSP -|- a.
+    Proof.
+      clear - BIL IL; intros.
+      rewrite sepSPC. rewrite empSPL. reflexivity.
+    Qed.
+
+    Lemma Sem_equiv_e_true_e_and_unitLL
+    : forall a : expr sym,
+        Sem_equiv _ SL lequiv (e_and e_true a) a.
+    Proof.
+      red; intros.
+      destruct (e_trueOk us tvs) as [ ? [ ? ? ] ].
+      consider (exprD' us tvs a SL); intros; repeat go_crazy; auto.
+      inv_all; subst; intros.
+      Cases.rewrite_all. clear - IL.
+      rewrite ltrue_unitL. reflexivity.
+    Qed.
+
+    Lemma Sem_equiv_e_true_e_and_unitLR
+    : forall a : expr sym,
+        Sem_equiv _ SL lequiv (e_and a e_true) a.
+    Proof.
+      red; intros.
+      destruct (e_trueOk us tvs) as [ ? [ ? ? ] ].
+      consider (exprD' us tvs a SL); intros; repeat go_crazy; auto.
+      inv_all; subst; intros.
+      Cases.rewrite_all. clear - IL.
+      rewrite ltrue_unitR. reflexivity.
+    Qed.
+    Lemma Sem_equiv_e_true_e_and_unitRL
+    : forall a : expr sym,
+        Sem_equiv _ SL lequiv a (e_and e_true a).
+    Proof.
+      red; intros.
+      destruct (e_trueOk us tvs) as [ ? [ ? ? ] ].
+      consider (exprD' us tvs a SL); intros; repeat go_crazy; auto.
+      inv_all; subst; intros.
+      Cases.rewrite_all. clear - IL.
+      rewrite ltrue_unitL. reflexivity.
+    Qed.
+    Lemma Sem_equiv_e_true_e_and_unitRR
+    : forall a : expr sym,
+        Sem_equiv _ SL lequiv a (e_and a e_true).
+    Proof.
+      red; intros.
+      destruct (e_trueOk us tvs) as [ ? [ ? ? ] ].
+      consider (exprD' us tvs a SL); intros; repeat go_crazy; auto.
+      inv_all; subst; intros.
+      Cases.rewrite_all. clear - IL.
+      rewrite ltrue_unitR. reflexivity.
+    Qed.
+
+    Lemma Sem_equiv_e_emp_e_star_unitLL
+    : forall a : expr sym,
+        Sem_equiv _ SL lequiv (e_star e_emp a) a.
+    Proof.
+      red; intros.
+      destruct (e_empOk us tvs) as [ ? [ ? ? ] ].
+      consider (exprD' us tvs a SL); intros; repeat go_crazy; auto.
+      inv_all; subst; intros.
+      Cases.rewrite_all. clear - BIL IL.
+      rewrite empSPL. reflexivity.
+    Qed.
+    Lemma Sem_equiv_e_emp_e_star_unitLR
+    : forall a : expr sym,
+        Sem_equiv _ SL lequiv (e_star a e_emp) a.
+    Proof.
+      red; intros.
+      destruct (e_empOk us tvs) as [ ? [ ? ? ] ].
+      consider (exprD' us tvs a SL); intros; repeat go_crazy; auto.
+      inv_all; subst; intros.
+      Cases.rewrite_all. clear - BIL.
+      rewrite empSPR. reflexivity.
+    Qed.
+    Lemma Sem_equiv_e_emp_e_star_unitRL
+    : forall a : expr sym,
+        Sem_equiv _ SL lequiv a (e_star e_emp a).
+    Proof.
+      red; intros.
+      destruct (e_empOk us tvs) as [ ? [ ? ? ] ].
+      consider (exprD' us tvs a SL); intros; repeat go_crazy; auto.
+      inv_all; subst; intros.
+      Cases.rewrite_all. clear - BIL.
+      rewrite empSPL. reflexivity.
+    Qed.
+    Lemma Sem_equiv_e_emp_e_star_unitRR
+    : forall a : expr sym,
+        Sem_equiv _ SL lequiv a (e_star a e_emp).
+    Proof.
+      red; intros.
+      destruct (e_empOk us tvs) as [ ? [ ? ? ] ].
+      consider (exprD' us tvs a SL); intros; repeat go_crazy; auto.
+      inv_all; subst; intros.
+      Cases.rewrite_all. clear - BIL.
+      rewrite empSPR. reflexivity.
+    Qed.
+
+    Local Instance PureOp_it : @PureOp _  := slsok.(_PureOp).
+    Local Instance Pure_it : @Pure _ _ _ slsok.(_PureOp) := _Pure slsok.
+
+    Lemma something_smart
+    : forall a b c d,
+        Pure.pure a -> Pure.pure b ->
+        (a //\\ b) //\\ c ** d -|- (a //\\ c) ** b //\\ d.
+    Proof.
+      clear - BIL IL. intros.
+      symmetry.
+      rewrite pureandscD by eauto with typeclass_instances.
+      rewrite sepSPC.
+      rewrite pureandscD by eauto with typeclass_instances.
+      rewrite <- landA.
+      rewrite sepSPC. reflexivity.
+    Qed.
+
+    Lemma well_formed_pure
+    : forall x us tvs (vs : hlist _ tvs),
+        well_formed x us (join_env vs) ->
+        forall x7,
+          exprD' us tvs (iterated_base e_true e_and (pure x)) SL = Some x7 ->
+          Pure.pure (x7 vs).
+    Proof.
+      unfold well_formed. destruct x; simpl.
+      induction 1; simpl; intros.
+      { unfold iterated_base in H. simpl in *.
+        destruct (e_trueOk us tvs).
+        rewrite H in *. destruct H0.
+        inv_all; subst. rewrite H1.
+        eapply pure_ltrue; eauto with typeclass_instances. }
+      { unfold iterated_base in *. simpl in *.
+        destruct (iterated e_and l); intros.
+        { go_crazy.
+          rewrite H3.
+          destruct H. destruct H.
+          eapply pure_land; eauto with typeclass_instances.
+          unfold exprD in *. rewrite split_env_join_env in *.
+          rewrite H1 in *. inv_all. rewrite H. auto. }
+        { destruct H. destruct H.
+          unfold exprD in H. rewrite split_env_join_env in *.
+          rewrite H1 in *. inv_all; subst.
+          auto. } }
+    Qed.
+
+    Lemma Forall_app : forall T (P : T -> Prop) xs ys,
+                         List.Forall P (xs ++ ys) <-> (List.Forall P xs /\ List.Forall P ys).
+    Proof.
+      clear. induction xs; simpl; intros.
+      { intuition. }
+      { split; intros.
+        { inversion H; subst. rewrite IHxs in H3. intuition. }
+        { intuition. inversion H0; subst. constructor; eauto. eapply IHxs. auto. } }
+    Qed.
+
+    Lemma cte_mkStar
+    : forall us tvs r_res l_res rval lval,
+        exprD' us tvs (conjunctives_to_expr r_res) SL = Some rval ->
+        exprD' us tvs (conjunctives_to_expr l_res) SL = Some lval ->
+        exists val,
+          exprD' us tvs (conjunctives_to_expr (mkStar l_res r_res)) SL = Some val /\
+          forall vs,
+            well_formed l_res us (join_env vs) ->
+            well_formed r_res us (join_env vs) ->
+            (val vs -|- lval vs ** rval vs) /\
+            well_formed (mkStar l_res r_res) us (join_env vs).
+    Proof.
+      intros.
+      specialize (conjunctives_to_expr_conjunctives_to_expr' r_res us tvs).
+      specialize (conjunctives_to_expr_conjunctives_to_expr' l_res us tvs).
+      specialize (conjunctives_to_expr_conjunctives_to_expr' (mkStar l_res r_res) us tvs).
+      About Reflexive_Sem_equiv.
+      generalize (@iterated_base_app _ e_true e_and (Sem_equiv _ SL lequiv)
+                                     (@Reflexive_Sem_equiv _ _ _ SL lequiv _)
+                                     (@Transitive_Sem_equiv _ _ _ SL lequiv _)
+                                     Sem_equiv_e_and_assoc Sem_equiv_Proper_e_and
+                 Sem_equiv_e_true_e_and_unitLL
+                 Sem_equiv_e_true_e_and_unitLR
+                 Sem_equiv_e_true_e_and_unitRL
+                 Sem_equiv_e_true_e_and_unitRR r_res.(pure) l_res.(pure) us tvs).
+(*
+      generalize (@iterated_base_app _ e_emp e_star (Sem_equiv _ SL lequiv) _ _
+                                     Sem_equiv_e_star_assoc Sem_equiv_Proper_e_star
+                 Sem_equiv_e_emp_e_star_unitLL
+                 Sem_equiv_e_emp_e_star_unitLR
+                 Sem_equiv_e_emp_e_star_unitRL
+                 Sem_equiv_e_emp_e_star_unitRR (map
+                (fun x : expr sym * list (expr sym) => apps (fst x) (snd x))
+                (spatial r_res)) (map
+                (fun x : expr sym * list (expr sym) => apps (fst x) (snd x))
+                (spatial l_res)) us tvs).
+ *)
+      Cases.rewrite_all_goal.
+      unfold Sem_equiv, mkStar, conjunctives_to_expr', conjunctives_to_expr; simpl.
+      clear H H0; intros; forward.
+      repeat go_crazy.
+      inv_all; subst.
+      forward. 
+      repeat go_crazy.
+      admit.
+(*
+      destruct (spatial l_res).
+      { destruct (spatial r_res).
+
+      match goal with
+        | |- exists x, exprD' _ _ ?X _ = _ /\ _ =>
+          generalize dependent X
+      end.
+      intros.
+      consider (exprD' us tvs e SL); intros; forward.
+      { eexists; split; eauto.
+        intros. split.
+        rewrite H4 , 
+                 
+      generalize dependent (match
+                               match spatial l_res with
+                                 | Some a =>
+                                   match spatial r_res with
+                                     | Some b => Some (a ++ b)
+                                     | None => Some a
+                                   end
+                                 | None => spatial r_res
+                               end
+                             with
+                               | Some s =>
+                                 match iterated e_and (pure l_res ++ pure r_res) with
+                                   | Some p =>
+                                     e_and p
+                                           (iterated_base e_emp e_star
+                                                          (map
+                                                             (fun x : expr sym * list (expr sym) =>
+                                                                apps (fst x) (snd x)) s))
+                                   | None =>
+                                     iterated_base e_emp e_star
+                                                   (map
+                                                      (fun x : expr sym * list (expr sym) =>
+                                                         apps (fst x) (snd x)) s)
+                                 end
+                               | None => iterated_base e_true e_and (pure l_res ++ pure r_res)
+                             end); 
+      
+
+
+      destruct (l_res.(spatial)); destruct (r_res.(spatial)).
+      { generalize (
+      inv_all; subst.
+      consider (iterated e_and (pure l_res ++ pure r_res)); intros.
+      { forward. repeat go_crazy.
+        inv_all; subst.
+        eexists; split; eauto.
+        intros.
+        unfold iterated_base in H0. rewrite H1 in H0.
+        rewrite H0 in H14. inv_all; subst.
+        split.
+        { rewrite H4 , H5. rewrite H9 , H7 , H21.
+          rewrite H12. rewrite H11.
+          rewrite H10. rewrite H15.
+          eapply something_smart.
+          red in H20.
+          eapply well_formed_pure. 2: eauto. eauto.
+          eapply well_formed_pure. 2: eauto. eauto. }
+        { unfold well_formed; simpl.
+          rewrite Forall_app. split.
+          eapply H20. eapply H22. } }
+      { eapply iterated_None in H1. rewrite H1 in *.
+        unfold iterated_base in H0. simpl in H0.
+        repeat go_crazy.
+        eexists; split; eauto.
+        intros. unfold well_formed; simpl; split; auto.
+        rewrite H4 , H5 , H7. rewrite H14. rewrite H16. rewrite H9.
+        rewrite H10. rewrite H17. rewrite H12 , H11.
+        eapply something_smart.
+        clear - H1 H2 e_trueOk BIL IL.
+        unfold iterated_base in *.
+        destruct (pure l_res); simpl in *; try congruence.
+        specialize (e_trueOk us tvs). destruct e_trueOk. rewrite H2 in *.
+        destruct H. inv_all; subst.
+        rewrite H0. eapply pure_ltrue; eauto with typeclass_instances.
+        clear - H1 H3 e_trueOk BIL IL.
+        unfold iterated_base in *.
+        destruct (pure l_res); simpl in *; try congruence.
+        specialize (e_trueOk us tvs). rewrite H1 in *. simpl in *.
+        destruct e_trueOk. rewrite H3 in *.
+        destruct H. inv_all; subst.
+        rewrite H0. eapply pure_ltrue; eauto with typeclass_instances. }
+*)
+    Qed.
+
+(*
+    Lemma cte_mkStar
+    : forall us tvs r_res l_res rval lval val,
+        exprD' us tvs (conjunctives_to_expr r_res) SL = Some rval ->
+        exprD' us tvs (conjunctives_to_expr l_res) SL = Some lval ->
+        exprD' us tvs (conjunctives_to_expr (mkStar l_res r_res)) SL = Some val ->
+        forall vs, val vs -|- lval vs ** rval vs.
+    Proof.
+      intros.
+      specialize (conjunctives_to_expr_conjunctives_to_expr' r_res us tvs).
+      specialize (conjunctives_to_expr_conjunctives_to_expr' l_res us tvs).
+      specialize (conjunctives_to_expr_conjunctives_to_expr' (mkStar l_res r_res) us tvs).
+      Cases.rewrite_all_goal.
+      unfold mkStar, conjunctives_to_expr'; simpl.
+      clear H H0 H1; intros; forward.
+      rewrite map_app in *.
+      generalize dependent (map
+                (fun x : expr sym * list (expr sym) => apps (fst x) (snd x))
+                (spatial l_res)).
+      generalize dependent (map (fun x : expr sym * list (expr sym) => apps (fst x) (snd x))
+               (spatial r_res)); intros.
+      assert (forall a b c : expr sym,
+                Sem_equiv SL lequiv (e_and a (e_and b c)) (e_and (e_and a b) c)).
+      { clear - IL e_andOk e_andValid. intros.
+        red. intros.
+        consider (exprD' us tvs (e_and a (e_and b c)) SL);
+          consider (exprD' us tvs (e_and (e_and a b) c) SL); intros; auto.
+        { eapply e_andValid in H. eapply e_andValid in H0.
+          do 2 destruct H; do 2 destruct H0.
+          destruct H0. destruct H1. destruct H. destruct H3.
+          eapply e_andValid in H. do 3 destruct H. destruct H5.
+          eapply e_andValid in H1. do 3 destruct H1. destruct H7.
+          rewrite H4. rewrite H2. rewrite H6. rewrite H8.
+          rewrite H0 in *. rewrite H5 in *. rewrite H7 in *.
+          inv_all; subst.
+          symmetry. eapply landA. }
+        { eapply e_andValid in H0.
+          do 3 destruct H0. destruct H1.
+          eapply e_andValid in H1.
+          do 3 destruct H1. destruct H3.
+          destruct (@e_andOk _ _ _ _ _ _ H0 H1). destruct H5.
+          destruct (@e_andOk _ _ _ _ _ _ H5 H3). destruct H7.
+          congruence. }
+        { eapply e_andValid in H.
+          do 3 destruct H. destruct H1.
+          eapply e_andValid in H.
+          do 3 destruct H. destruct H3.
+          destruct (@e_andOk _ _ _ _ _ _ H3 H1). destruct H5.
+          destruct (@e_andOk _ _ _ _ _ _ H H5). destruct H7.
+          congruence. } }
+      assert (Proper
+                (Sem_equiv SL lequiv ==> Sem_equiv SL lequiv ==> Sem_equiv SL lequiv)
+                e_and).
+      { clear - IL e_andOk e_andValid. intros.
+        repeat red; unfold Sem_equiv; intros.
+        specialize (H us tvs). specialize (H0 us tvs).
+        admit. }
+      assert (forall a : expr sym, Sem_equiv SL lequiv (e_and e_emp a) a) by admit.
+      assert (forall a : expr sym, Sem_equiv SL lequiv (e_and a e_emp) a) by admit.
+      assert (forall a : expr sym, Sem_equiv SL lequiv a (e_and e_emp a)) by admit.
+      assert (forall a : expr sym, Sem_equiv SL lequiv a (e_and a e_emp)) by admit.
+      eapply e_starValid in H1. eapply e_starValid in H0. eapply e_starValid in H.
+      repeat match goal with
+               | H : exists x, _ |- _ => destruct H
+               | H : _ /\ _ |- _ => destruct H
+             end.
+      specialize (@iterated_base_app (expr sym) e_emp e_and (@Sem_equiv SL lequiv) _ _ H5 H6 H7 H8 H9 H10 
+                                     (pure r_res) (pure l_res) us tvs).
+      rewrite H.
+      destruct (@e_andOk us tvs _ _ _ _ H0 H1). destruct H17. rewrite H17; intros.
+      assert (forall a : expr sym, Sem_equiv SL lequiv (e_star e_emp a) a) by admit.
+      assert (forall a : expr sym, Sem_equiv SL lequiv (e_star a e_emp) a) by admit.
+      assert (forall a : expr sym, Sem_equiv SL lequiv a (e_star e_emp a)) by admit.
+      assert (forall a : expr sym, Sem_equiv SL lequiv a (e_star a e_emp)) by admit.
+      assert (forall a b c : expr sym,
+                Sem_equiv SL lequiv (e_star a (e_star b c)) (e_star (e_star a b) c)).
+      { clear - IL BIL e_starOk e_starValid. intros.
+        red. intros.
+        consider (exprD' us tvs (e_star a (e_star b c)) SL);
+          consider (exprD' us tvs (e_star (e_star a b) c) SL); intros; auto.
+        { eapply e_starValid in H. eapply e_starValid in H0.
+          do 2 destruct H; do 2 destruct H0.
+          destruct H0. destruct H1. destruct H. destruct H3.
+          eapply e_starValid in H. do 3 destruct H. destruct H5.
+          eapply e_starValid in H1. do 3 destruct H1. destruct H7.
+          rewrite H4. rewrite H2. rewrite H6. rewrite H8.
+          rewrite H in *. rewrite H1 in *. rewrite H7 in *.
+          inv_all; subst. rewrite sepSPA. reflexivity. }
+        { eapply e_starValid in H0.
+          do 3 destruct H0. destruct H1.
+          eapply e_starValid in H1.
+          do 3 destruct H1. destruct H3.
+          destruct (@e_starOk _ _ _ _ _ _ H0 H1). destruct H5.
+          destruct (@e_starOk _ _ _ _ _ _ H5 H3). destruct H7.
+          congruence. }
+        { eapply e_starValid in H.
+          do 3 destruct H. destruct H1.
+          eapply e_starValid in H.
+          do 3 destruct H. destruct H3.
+          destruct (@e_starOk _ _ _ _ _ _ H3 H1). destruct H5.
+          destruct (@e_starOk _ _ _ _ _ _ H H5). destruct H7.
+          congruence. } }
+      assert (Proper
+                (Sem_equiv SL lequiv ==> Sem_equiv SL lequiv ==> Sem_equiv SL lequiv)
+                e_star) by admit.
+      specialize (@iterated_base_app (expr sym) e_emp e_star (@Sem_equiv SL lequiv) _ _ H24 H25 H20 H21 H22 H23
+                                     l l0 us tvs).
+      rewrite H11.
+      destruct (@e_starOk us tvs _ _ _ _ H13 H15). destruct H26. rewrite H26; intros.
+      rewrite H4 , H3 , H2 , H12 , H14 , H16.
+      rewrite H28 , H19 , H18. rewrite H27.
+      admit.
+    Qed.
+*)
+
+
+    Theorem SepLogArgsOk_conjunctives : SepLogArgsOk RSym_sym SL SepLogArgs_normalize SLS R_conjunctives.
+    Proof.
+      constructor; unfold R_conjunctives; simpl; intros.
+      { unfold mkSpatial, conjunctives_to_expr. simpl.
+        eexists; split; eauto.
+        split. reflexivity; intros.
+        intuition. red. simpl. constructor. }
+      { unfold conjunctives_to_expr, mkPure; simpl.
+        unfold iterated_base. simpl.
+        eexists; split; eauto; intros.
+        split; auto.
+        red. simpl. constructor; auto.
+        unfold exprD. rewrite split_env_join_env. rewrite H1.
+        eexists; split; eauto.
+        eapply His_pure in H0.
+        eapply H0.
+        instantiate (1 := join_env vs).
+        instantiate (1 := join_env us).
+        unfold exprD. rewrite split_env_join_env. rewrite H1. reflexivity. }
+      { unfold conjunctives_to_expr, mkEmpty; simpl.
+        specialize (e_empOk (join_env us) tvs). destruct e_empOk; clear e_empOk.
+        destruct H2. eexists; split; eauto.
+        split; intros.
+        rewrite H3. generalize (slsok.(His_emp) _ H0 (join_env us) (join_env vs)).
+        unfold exprD. rewrite split_env_join_env. rewrite H1. intros.
+        inv_all. rewrite H4. reflexivity.
+        red; simpl. constructor. }
+      { red_exprD.
+        generalize (slsok.(His_star) _ H2 (join_env us)).
+        unfold type_of_apply in *.
+        forward. inv_all; subst. inv_all. subst t0 t5. clear H5.
+        unfold mkStar, conjunctives_to_expr. simpl.
+        red_exprD. forward. inv_all; subst.
+        specialize (H3 _ _ H10).
+        specialize (H4 _ _ H9).
+        destruct H3. destruct H4.
+        destruct H , H3.
+        destruct (@cte_mkStar (join_env us) tvs _ _ _ _ H3 H).
+        destruct H11. unfold mkStar in H11. unfold conjunctives_to_expr in H11.
+        simpl in H11.
+        eexists; split; eauto.
+        uip_all'. simpl in *.
+        specialize (H4 vs); specialize (H6 vs).
+        destruct H4 , H6.
+        destruct (H13 vs H14 H15).
+        split.
+        { eapply His_star in H2; eauto with typeclass_instances.
+          revert H2.
+          instantiate (1 := join_env vs).
+          instantiate (1 := join_env us).
+          intros. unfold exprD in H2. rewrite split_env_join_env in H2.
+          rewrite H8 in *. inv_all. rewrite H2.
+          rewrite H16. rewrite H4 , H6. reflexivity. }
+        { eapply H17. } }
+    Qed.
+
+  End conjunctivesD.
+
+(*
+  Section demo.
+  Definition is_emp (i : sym) : bool :=
     match i with
       | ilf_true _ => true
       | _ => false
     end.
-  Definition is_star (e : expr ilfunc) : bool :=
+  Definition is_star (e : expr sym) : bool :=
     match e with
       | Inj (fref 1%positive) => true
       | _ => false
     end.
 
-  Definition normalizeArgs : AppFullFoldArgs ilfunc conjunctives :=
-  {| do_var := fun v _ _ => atomic (Var v)
-   ; do_uvar := fun u _ _ => atomic (UVar u)
-   ; do_inj := fun i _ _ => if is_emp i then empty else atomic (Inj i)
-   ; do_abs := fun t e _ _ _ => atomic (Abs t e)
-   ; do_app := fun f _ args tus tvs =>
-                 if is_star f then
-                   match args with
-                     | (_,l) :: (_,r) :: nil =>
-                       join (l tus tvs) (r tus tvs)
-                     | _ => empty
-                   end
-                 else
-                   atomic_app f (map fst args)
-  |}.
 
-  Section demo.
     Definition inj_emp := Inj (ilf_true (tyType 0)).
     Definition inj_star a b :=
       Eval compute in apps (Inj (fref 1%positive)) (a :: b :: nil).
@@ -68,6 +1010,7 @@ Section cancel_state.
     Eval compute in  test (inj_star inj_emp inj_emp).
     Eval compute in  test (inj_star (Var 0) (inj_star inj_emp (inj_and (Var 1) (Var 3)))).
   End demo.
+*)
 
   Require Import ExtLib.Structures.Monads.
   Require Import ExtLib.Data.Monads.StateMonad.
@@ -79,6 +1022,7 @@ Section cancel_state.
     Definition conjunctives_remove (c : conjunctives) (e : expr ilfunc)
     : option conjunctives:= None.
 
+(*
   Definition cancel_atomic (e : expr ilfunc) : state conjunctives conjunctives :=
     (lhs <- get ;;
      match conjunctives_remove lhs e with
@@ -97,6 +1041,7 @@ Section cancel_state.
 
 
   Definition cancel (rhs : expr ilfunc) : conjunctives -> (conjunctives * conjunctives).
-
+*)
+  End with_monad.
 
 End cancel_state.
